cfrontend/Cop.v
@@ -238,7 +238,7 @@ Definition sem_cast (v: val) (t1 t2: type) (m: mem): option val :=
   match classify_cast t1 t2 with
   | cast_case_pointer =>
       match v with
-      | Vptr _ _ => Some v
+      | Vfptr _ => Some v
       | Vint _ => if Archi.ptr64 then None else Some v
       | Vlong _ => if Archi.ptr64 then Some v else None
       | _ => None
@@ -300,19 +300,12 @@ Definition sem_cast (v: val) (t1 t2: type) (m: mem): option val :=
       match v with
       | Vint n =>
           Some(Vint(if Int.eq n Int.zero then Int.zero else Int.one))
-      | Vptr b ofs =>
-          if Archi.ptr64 then None else
-          if Mem.weak_valid_pointer m b (Ptrofs.unsigned ofs) then Some Vone else None
       | _ => None
       end
   | cast_case_l2bool =>
       match v with
       | Vlong n =>
           Some(Vint(if Int64.eq n Int64.zero then Int.zero else Int.one))
-      | Vptr b ofs =>
-          if negb Archi.ptr64 then None else
-          if Mem.weak_valid_pointer m b (Ptrofs.unsigned ofs) then Some Vone else None
-
       | _ => None
       end
   | cast_case_f2bool =>
@@ -372,13 +365,13 @@ Definition sem_cast (v: val) (t1 t2: type) (m: mem): option val :=
       end
   | cast_case_struct id1 id2 =>
       match v with
-      | Vptr b ofs =>
+      | Vint ofs =>
           if ident_eq id1 id2 then Some v else None
       | _ => None
       end
   | cast_case_union id1 id2 =>
       match v with
-      | Vptr b ofs =>
+      | Vint ofs =>
           if ident_eq id1 id2 then Some v else None
       | _ => None
       end
@@ -420,17 +413,13 @@ Definition bool_val (v: val) (t: type) (m: mem) : option bool :=
   | bool_case_i =>
       match v with
       | Vint n => Some (negb (Int.eq n Int.zero))
-      | Vptr b ofs =>
-          if Archi.ptr64 then None else
-          if Mem.weak_valid_pointer m b (Ptrofs.unsigned ofs) then Some true else None
+      | Vfptr b => if Archi.ptr64 then None else Some true
       | _ => None
       end
   | bool_case_l =>
       match v with
       | Vlong n => Some (negb (Int64.eq n Int64.zero))
-      | Vptr b ofs =>
-          if negb Archi.ptr64 then None else
-          if Mem.weak_valid_pointer m b (Ptrofs.unsigned ofs) then Some true else None
+      | Vfptr b => if negb Archi.ptr64 then None else Some true
       | _ => None
       end
   | bool_case_f =>
@@ -662,9 +651,7 @@ Definition ptrofs_of_int (si: signedness) (n: int) : ptrofs :=
 
 Definition sem_add_ptr_int (cenv: composite_env) (ty: type) (si: signedness) (v1 v2: val): option val :=
   match v1, v2 with
-  | Vptr b1 ofs1, Vint n2 =>
-      let n2 := ptrofs_of_int si n2 in
-      Some (Vptr b1 (Ptrofs.add ofs1 (Ptrofs.mul (Ptrofs.repr (sizeof cenv ty)) n2)))
+  | Vfptr b1, Vint n2 => None
   | Vint n1, Vint n2 =>
       if Archi.ptr64 then None else Some (Vint (Int.add n1 (Int.mul (Int.repr (sizeof cenv ty)) n2)))
   | Vlong n1, Vint n2 =>
@@ -675,9 +662,7 @@ Definition sem_add_ptr_int (cenv: composite_env) (ty: type) (si: signedness) (v1
 
 Definition sem_add_ptr_long (cenv: composite_env) (ty: type) (v1 v2: val): option val :=
   match v1, v2 with
-  | Vptr b1 ofs1, Vlong n2 =>
-      let n2 := Ptrofs.of_int64 n2 in
-      Some (Vptr b1 (Ptrofs.add ofs1 (Ptrofs.mul (Ptrofs.repr (sizeof cenv ty)) n2)))
+  | Vfptr b1, Vlong n2 => None
   | Vint n1, Vlong n2 =>
       let n2 := Int.repr (Int64.unsigned n2) in
       if Archi.ptr64 then None else Some (Vint (Int.add n1 (Int.mul (Int.repr (sizeof cenv ty)) n2)))
@@ -725,9 +710,7 @@ Definition sem_sub (cenv: composite_env) (v1:val) (t1:type) (v2: val) (t2:type) 
   match classify_sub t1 t2 with
   | sub_case_pi ty si =>            (**r pointer minus integer *)
       match v1, v2 with
-      | Vptr b1 ofs1, Vint n2 =>
-          let n2 := ptrofs_of_int si n2 in
-          Some (Vptr b1 (Ptrofs.sub ofs1 (Ptrofs.mul (Ptrofs.repr (sizeof cenv ty)) n2)))
+      | Vfptr b1, Vint n2 => None
       | Vint n1, Vint n2 =>
           if Archi.ptr64 then None else Some (Vint (Int.sub n1 (Int.mul (Int.repr (sizeof cenv ty)) n2)))
       | Vlong n1, Vint n2 =>
@@ -737,9 +720,7 @@ Definition sem_sub (cenv: composite_env) (v1:val) (t1:type) (v2: val) (t2:type) 
       end
   | sub_case_pl ty =>            (**r pointer minus long *)
       match v1, v2 with
-      | Vptr b1 ofs1, Vlong n2 =>
-          let n2 := Ptrofs.of_int64 n2 in
-          Some (Vptr b1 (Ptrofs.sub ofs1 (Ptrofs.mul (Ptrofs.repr (sizeof cenv ty)) n2)))
+      | Vfptr b1, Vlong n2 => None
       | Vint n1, Vlong n2 =>
           let n2 := Int.repr (Int64.unsigned n2) in
           if Archi.ptr64 then None else Some (Vint (Int.sub n1 (Int.mul (Int.repr (sizeof cenv ty)) n2)))
@@ -749,13 +730,8 @@ Definition sem_sub (cenv: composite_env) (v1:val) (t1:type) (v2: val) (t2:type) 
       end
   | sub_case_pp ty =>          (**r pointer minus pointer *)
       match v1,v2 with
-      | Vptr b1 ofs1, Vptr b2 ofs2 =>
-          if eq_block b1 b2 then
-            let sz := sizeof cenv ty in
-            if zlt 0 sz && zle sz Ptrofs.max_signed
-            then Some (Vptrofs (Ptrofs.divs (Ptrofs.sub ofs1 ofs2) (Ptrofs.repr sz)))
-            else None
-          else None
+      | Vfptr b1, Vfptr b2 =>
+          if eq_block b1 b2 then Some Vzero else None
       | _, _ => None
       end
   | sub_default =>
@@ -948,8 +924,8 @@ Definition classify_cmp (ty1: type) (ty2: type) :=
 Definition cmp_ptr (m: mem) (c: comparison) (v1 v2: val): option val :=
   option_map Val.of_bool
    (if Archi.ptr64
-    then Val.cmplu_bool (Mem.valid_pointer m) c v1 v2
-    else Val.cmpu_bool (Mem.valid_pointer m) c v1 v2).
+    then Val.cmplu_bool c v1 v2
+    else Val.cmpu_bool c v1 v2).
 
 Definition sem_cmp (c:comparison)
                   (v1: val) (t1: type) (v2: val) (t2: type)
@@ -962,7 +938,7 @@ Definition sem_cmp (c:comparison)
       | Vint n2 =>
           let v2' := Vptrofs (ptrofs_of_int si n2) in
           cmp_ptr m c v1 v2'
-      | Vptr b ofs =>
+      | Vfptr b =>
           if Archi.ptr64 then None else cmp_ptr m c v1 v2
       | _ =>
           None
@@ -972,7 +948,7 @@ Definition sem_cmp (c:comparison)
       | Vint n1 =>
           let v1' := Vptrofs (ptrofs_of_int si n1) in
           cmp_ptr m c v1' v2
-      | Vptr b ofs =>
+      | Vfptr b =>
           if Archi.ptr64 then None else cmp_ptr m c v1 v2
       | _ =>
           None
@@ -982,7 +958,7 @@ Definition sem_cmp (c:comparison)
       | Vlong n2 =>
           let v2' := Vptrofs (Ptrofs.of_int64 n2) in
           cmp_ptr m c v1 v2'
-      | Vptr b ofs =>
+      | Vfptr b =>
           if Archi.ptr64 then cmp_ptr m c v1 v2 else None
       | _ =>
           None
@@ -992,7 +968,7 @@ Definition sem_cmp (c:comparison)
       | Vlong n1 =>
           let v1' := Vptrofs (Ptrofs.of_int64 n1) in
           cmp_ptr m c v1' v2
-      | Vptr b ofs =>
+      | Vfptr b =>
           if Archi.ptr64 then cmp_ptr m c v1 v2 else None
       | _ =>
           None
@@ -1152,287 +1128,6 @@ Inductive store_bitfield: type -> intsize -> signedness -> Z -> Z -> mem -> atom
       store_bitfield (Tint sz sg1 attr) sz sg pos width m (addr,pt) (Vint n,vt) lts
                      m' (Vint (bitfield_normalize sz sg width n),vt).
 
-(** * Compatibility with extensions and injections *)
-
-Section GENERIC_INJECTION.
-
-Variable f: meminj.
-Variables m m': mem.
-
-Hypothesis valid_pointer_inj:
-  forall b1 ofs b2 delta,
-  f b1 = Some(b2, delta) ->
-  Mem.valid_pointer m b1 (Ptrofs.unsigned ofs) = true ->
-  Mem.valid_pointer m' b2 (Ptrofs.unsigned (Ptrofs.add ofs (Ptrofs.repr delta))) = true.
-
-Hypothesis weak_valid_pointer_inj:
-  forall b1 ofs b2 delta,
-  f b1 = Some(b2, delta) ->
-  Mem.weak_valid_pointer m b1 (Ptrofs.unsigned ofs) = true ->
-  Mem.weak_valid_pointer m' b2 (Ptrofs.unsigned (Ptrofs.add ofs (Ptrofs.repr delta))) = true.
-
-Hypothesis weak_valid_pointer_no_overflow:
-  forall b1 ofs b2 delta,
-  f b1 = Some(b2, delta) ->
-  Mem.weak_valid_pointer m b1 (Ptrofs.unsigned ofs) = true ->
-  0 <= Ptrofs.unsigned ofs + Ptrofs.unsigned (Ptrofs.repr delta) <= Ptrofs.max_unsigned.
-
-Hypothesis valid_different_pointers_inj:
-  forall b1 ofs1 b2 ofs2 b1' delta1 b2' delta2,
-  b1 <> b2 ->
-  Mem.valid_pointer m b1 (Ptrofs.unsigned ofs1) = true ->
-  Mem.valid_pointer m b2 (Ptrofs.unsigned ofs2) = true ->
-  f b1 = Some (b1', delta1) ->
-  f b2 = Some (b2', delta2) ->
-  b1' <> b2' \/
-  Ptrofs.unsigned (Ptrofs.add ofs1 (Ptrofs.repr delta1)) <> Ptrofs.unsigned (Ptrofs.add ofs2 (Ptrofs.repr delta2)).
-
-Remark val_inject_vtrue: forall f, Val.inject f Vtrue Vtrue.
-Proof. unfold Vtrue; auto. Qed.
-
-Remark val_inject_vfalse: forall f, Val.inject f Vfalse Vfalse.
-Proof. unfold Vfalse; auto. Qed.
-
-Remark val_inject_of_bool: forall f b, Val.inject f (Val.of_bool b) (Val.of_bool b).
-Proof. intros. unfold Val.of_bool. destruct b; [apply val_inject_vtrue|apply val_inject_vfalse].
-Qed.
-
-Remark val_inject_vptrofs: forall n, Val.inject f (Vptrofs n) (Vptrofs n).
-Proof. intros. unfold Vptrofs. destruct Archi.ptr64; auto. Qed.
-
-Local Hint Resolve val_inject_vtrue val_inject_vfalse val_inject_of_bool val_inject_vptrofs : core.
-
-Ltac TrivialInject :=
-  match goal with
-  | [ H: None = Some _ |- _ ] => discriminate
-  | [ H: Some _ = Some _ |- _ ] => inv H; TrivialInject
-  | [ H: match ?x with Some _ => _ | None => _ end = Some _ |- _ ] => destruct x; TrivialInject
-  | [ H: match ?x with true => _ | false => _ end = Some _ |- _ ] => destruct x eqn:?; TrivialInject
-  | [ |- exists v', Some ?v = Some v' /\ _ ] => exists v; split; auto
-  | _ => idtac
-  end.
-
-Lemma sem_cast_inj:
-  forall v1 ty1 ty v tv1,
-  sem_cast v1 ty1 ty m = Some v ->
-  Val.inject f v1 tv1 ->
-  exists tv, sem_cast tv1 ty1 ty m'= Some tv /\ Val.inject f v tv.
-Proof.
-  unfold sem_cast; intros; destruct (classify_cast ty1 ty); inv H0; TrivialInject.
-- econstructor; eauto.
-- erewrite weak_valid_pointer_inj by eauto. TrivialInject. 
-- erewrite weak_valid_pointer_inj by eauto. TrivialInject. 
-- destruct (ident_eq id1 id2); TrivialInject. econstructor; eauto.
-- destruct (ident_eq id1 id2); TrivialInject. econstructor; eauto.
-- econstructor; eauto.
-Qed.
-
-Lemma bool_val_inj:
-  forall v ty b tv,
-  bool_val v ty m = Some b ->
-  Val.inject f v tv ->
-  bool_val tv ty m' = Some b.
-Proof.
-  unfold bool_val; intros.
-  destruct (classify_bool ty); inv H0; try congruence.
-  destruct Archi.ptr64; try discriminate.
-  destruct (Mem.weak_valid_pointer m b1 (Ptrofs.unsigned ofs1)) eqn:VP; inv H.
-  erewrite weak_valid_pointer_inj by eauto. auto.
-  destruct Archi.ptr64; try discriminate.
-  destruct (Mem.weak_valid_pointer m b1 (Ptrofs.unsigned ofs1)) eqn:VP; inv H.
-  erewrite weak_valid_pointer_inj by eauto. auto.
-Qed.
-
-Lemma sem_unary_operation_inj:
-  forall op v1 ty v tv1,
-  sem_unary_operation op v1 ty m = Some v ->
-  Val.inject f v1 tv1 ->
-  exists tv, sem_unary_operation op tv1 ty m' = Some tv /\ Val.inject f v tv.
-Proof.
-  unfold sem_unary_operation; intros. destruct op.
-- (* notbool *)
-  unfold sem_notbool in *. destruct (bool_val v1 ty m) as [b|] eqn:BV; simpl in H; inv H.
-  erewrite bool_val_inj by eauto. simpl. TrivialInject.
-- (* notint *)
-  unfold sem_notint in *; destruct (classify_notint ty); inv H0; inv H; TrivialInject.
-- (* neg *)
-  unfold sem_neg in *; destruct (classify_neg ty); inv H0; inv H; TrivialInject.
-- (* absfloat *)
-  unfold sem_absfloat in *; destruct (classify_neg ty); inv H0; inv H; TrivialInject.
-Qed.
-
-Definition optval_self_injects (ov: option val) : Prop :=
-  match ov with
-  | Some (Vptr b ofs) => False
-  | _ => True
-  end.
-
-Remark sem_binarith_inject:
-  forall sem_int sem_long sem_float sem_single v1 t1 v2 t2 v v1' v2',
-  sem_binarith sem_int sem_long sem_float sem_single v1 t1 v2 t2 m = Some v ->
-  Val.inject f v1 v1' -> Val.inject f v2 v2' ->
-  (forall sg n1 n2, optval_self_injects (sem_int sg n1 n2)) ->
-  (forall sg n1 n2, optval_self_injects (sem_long sg n1 n2)) ->
-  (forall n1 n2, optval_self_injects (sem_float n1 n2)) ->
-  (forall n1 n2, optval_self_injects (sem_single n1 n2)) ->
-  exists v', sem_binarith sem_int sem_long sem_float sem_single v1' t1 v2' t2 m' = Some v' /\ Val.inject f v v'.
-Proof.
-  intros.
-  assert (SELF: forall ov v, ov = Some v -> optval_self_injects ov -> Val.inject f v v).
-  {
-    intros. subst ov; simpl in H7. destruct v0; contradiction || constructor.
-  }
-  unfold sem_binarith in *.
-  set (c := classify_binarith t1 t2) in *.
-  set (t := binarith_type c) in *.
-  destruct (sem_cast v1 t1 t m) as [w1|] eqn:C1; try discriminate.
-  destruct (sem_cast v2 t2 t m) as [w2|] eqn:C2; try discriminate.
-  exploit (sem_cast_inj v1); eauto. intros (w1' & C1' & INJ1).
-  exploit (sem_cast_inj v2); eauto. intros (w2' & C2' & INJ2).
-  rewrite C1'; rewrite C2'.
-  destruct c; inv INJ1; inv INJ2; discriminate || eauto.
-Qed.
-
-Remark sem_shift_inject:
-  forall sem_int sem_long v1 t1 v2 t2 v v1' v2',
-  sem_shift sem_int sem_long v1 t1 v2 t2 = Some v ->
-  Val.inject f v1 v1' -> Val.inject f v2 v2' ->
-  exists v', sem_shift sem_int sem_long v1' t1 v2' t2 = Some v' /\ Val.inject f v v'.
-Proof.
-  intros. exists v.
-  unfold sem_shift in *; destruct (classify_shift t1 t2); inv H0; inv H1; try discriminate.
-  destruct (Int.ltu i0 Int.iwordsize); inv H; auto.
-  destruct (Int64.ltu i0 Int64.iwordsize); inv H; auto.
-  destruct (Int64.ltu i0 (Int64.repr 32)); inv H; auto.
-  destruct (Int.ltu i0 Int64.iwordsize'); inv H; auto.
-Qed.
-
-Remark sem_cmp_ptr_inj:
-  forall c v1 v2 v tv1 tv2,
-  cmp_ptr m c v1 v2 = Some v ->
-  Val.inject f v1 tv1 ->
-  Val.inject f v2 tv2 ->
-  exists tv, cmp_ptr m' c tv1 tv2 = Some tv /\ Val.inject f v tv.
-Proof.
-  unfold cmp_ptr; intros. 
-  remember (if Archi.ptr64
-       then Val.cmplu_bool (Mem.valid_pointer m) c v1 v2
-       else Val.cmpu_bool (Mem.valid_pointer m) c v1 v2) as ob.
-  destruct ob as [b|]; simpl in H; inv H.
-  exists (Val.of_bool b); split; auto.
-  destruct Archi.ptr64. 
-  erewrite Val.cmplu_bool_inject by eauto. auto.
-  erewrite Val.cmpu_bool_inject by eauto. auto.
-Qed.
-
-Remark sem_cmp_inj:
-  forall cmp v1 tv1 ty1 v2 tv2 ty2 v,
-  sem_cmp cmp v1 ty1 v2 ty2 m = Some v ->
-  Val.inject f v1 tv1 ->
-  Val.inject f v2 tv2 ->
-  exists tv, sem_cmp cmp tv1 ty1 tv2 ty2 m' = Some tv /\ Val.inject f v tv.
-Proof.
-  intros.
-  unfold sem_cmp in *; destruct (classify_cmp ty1 ty2).
-- (* pointer - pointer *)
-  eapply sem_cmp_ptr_inj; eauto.
-- (* pointer - int *)
-  inversion H1; subst; TrivialInject; eapply sem_cmp_ptr_inj; eauto.
-- (* int - pointer *)
-  inversion H0; subst; TrivialInject; eapply sem_cmp_ptr_inj; eauto.
-- (* pointer - long *)
-  inversion H1; subst; TrivialInject; eapply sem_cmp_ptr_inj; eauto.
-- (* long - pointer *)
-  inversion H0; subst; TrivialInject; eapply sem_cmp_ptr_inj; eauto.
-- (* numerical - numerical *)
-  assert (SELF: forall b, optval_self_injects (Some (Val.of_bool b))).
-  {
-    destruct b; exact I.
-  }
-  eapply sem_binarith_inject; eauto.
-Qed.
-
-Lemma sem_binary_operation_inj:
-  forall cenv op v1 ty1 v2 ty2 v tv1 tv2,
-  sem_binary_operation cenv op v1 ty1 v2 ty2 m = Some v ->
-  Val.inject f v1 tv1 -> Val.inject f v2 tv2 ->
-  exists tv, sem_binary_operation cenv op tv1 ty1 tv2 ty2 m' = Some tv /\ Val.inject f v tv.
-Proof.
-  unfold sem_binary_operation; intros; destruct op.
-- (* add *)
-  assert (A: forall cenv ty si v1' v2' tv1' tv2',
-             Val.inject f v1' tv1' -> Val.inject f v2' tv2' ->
-             sem_add_ptr_int cenv ty si v1' v2' = Some v ->
-             exists tv, sem_add_ptr_int cenv ty si tv1' tv2' = Some tv /\ Val.inject f v tv).
-  { intros. unfold sem_add_ptr_int in *; inv H2; inv H3; TrivialInject.
-    econstructor. eauto. repeat rewrite Ptrofs.add_assoc. decEq. apply Ptrofs.add_commut. }
-  assert (B: forall cenv ty v1' v2' tv1' tv2',
-             Val.inject f v1' tv1' -> Val.inject f v2' tv2' ->
-             sem_add_ptr_long cenv ty v1' v2' = Some v ->
-             exists tv, sem_add_ptr_long cenv ty tv1' tv2' = Some tv /\ Val.inject f v tv).
-  { intros. unfold sem_add_ptr_long in *; inv H2; inv H3; TrivialInject.
-    econstructor. eauto. repeat rewrite Ptrofs.add_assoc. decEq. apply Ptrofs.add_commut. }
-  unfold sem_add in *; destruct (classify_add ty1 ty2); eauto.
-  + eapply sem_binarith_inject; eauto; intros; exact I.
-- (* sub *)
-  unfold sem_sub in *; destruct (classify_sub ty1 ty2).
-  + inv H0; inv H1; TrivialInject.
-    econstructor. eauto. rewrite Ptrofs.sub_add_l. auto. 
-  + inv H0; inv H1; TrivialInject.
-    destruct (eq_block b1 b0); try discriminate. subst b1.
-    rewrite H0 in H2; inv H2. rewrite dec_eq_true.
-    destruct (zlt 0 (sizeof cenv ty) && zle (sizeof cenv ty) Ptrofs.max_signed); inv H.
-    rewrite Ptrofs.sub_shifted. TrivialInject.
-  + inv H0; inv H1; TrivialInject.
-    econstructor. eauto. rewrite Ptrofs.sub_add_l. auto. 
-  + eapply sem_binarith_inject; eauto; intros; exact I.
-- (* mul *)
-  eapply sem_binarith_inject; eauto; intros; exact I.
-- (* div *)
-  eapply sem_binarith_inject; eauto; intros.
-  destruct sg.
-  destruct (Int.eq n2 Int.zero
-            || Int.eq n1 (Int.repr Int.min_signed) && Int.eq n2 Int.mone); exact I.
-  destruct (Int.eq n2 Int.zero); exact I.
-  destruct sg.
-  destruct (Int64.eq n2 Int64.zero
-            || Int64.eq n1 (Int64.repr Int64.min_signed) && Int64.eq n2 Int64.mone); exact I.
-  destruct (Int64.eq n2 Int64.zero); exact I.
-  exact I.
-  exact I.
-- (* mod *)
-  eapply sem_binarith_inject; eauto; intros.
-  destruct sg.
-  destruct (Int.eq n2 Int.zero
-            || Int.eq n1 (Int.repr Int.min_signed) && Int.eq n2 Int.mone); exact I.
-  destruct (Int.eq n2 Int.zero); exact I.
-  destruct sg.
-  destruct (Int64.eq n2 Int64.zero
-            || Int64.eq n1 (Int64.repr Int64.min_signed) && Int64.eq n2 Int64.mone); exact I.
-  destruct (Int64.eq n2 Int64.zero); exact I.
-  exact I.
-  exact I.
-- (* and *)
-  eapply sem_binarith_inject; eauto; intros; exact I.
-- (* or *)
-  eapply sem_binarith_inject; eauto; intros; exact I.
-- (* xor *)
-  eapply sem_binarith_inject; eauto; intros; exact I.
-- (* shl *)
-  eapply sem_shift_inject; eauto.
-- (* shr *)
-  eapply sem_shift_inject; eauto.
-  (* comparisons *)
-- eapply sem_cmp_inj; eauto.
-- eapply sem_cmp_inj; eauto.
-- eapply sem_cmp_inj; eauto.
-- eapply sem_cmp_inj; eauto.
-- eapply sem_cmp_inj; eauto.
-- eapply sem_cmp_inj; eauto.
-Qed.
-
-End GENERIC_INJECTION.
-
 (*Lemma sem_cast_inject:
   forall f v1 ty1 ty m v tv1 tm,
   sem_cast v1 ty1 ty m = Some v ->
@@ -1489,10 +1184,10 @@ Qed.*)
 
 (** Relation between Boolean value and casting to [_Bool] type. *)
 
-Lemma cast_bool_bool_val:
+(*Lemma cast_bool_bool_val:
   forall v t m,
-  sem_cast v t (Tint IBool Signed noattr) m =
-  match bool_val v t m with None => None | Some b => Some(Val.of_bool b) end.
+    sem_cast v t (Tint IBool Signed noattr) m =
+      match bool_val v t m with None => None | Some b => Some(Val.of_bool b) end.
   intros.
   assert (A: classify_bool t0 =
     match t0 with
@@ -1543,7 +1238,7 @@ Lemma cast_bool_bool_val:
   destruct ptr64; auto.
   destruct ptr64; auto. destruct (Mem.weak_valid_pointer m b (Ptrofs.unsigned i)); auto.
   destruct (Mem.weak_valid_pointer m b (Ptrofs.unsigned i)); auto.
-Qed.
+Qed.*)
 
 (** Relation between Boolean value and Boolean negation. *)
 
@@ -1569,20 +1264,16 @@ Inductive val_casted: val -> type -> Prop :=
        val_casted (Vsingle n) (Tfloat F32 attr)
   | val_casted_long: forall si attr n,
       val_casted (Vlong n) (Tlong si attr)
-  | val_casted_ptr_ptr: forall b ofs ty attr,
-      val_casted (Vptr b ofs) (Tpointer ty attr)
+  | val_casted_ptr_ptr: forall b ty attr,
+      val_casted (Vfptr b) (Tpointer ty attr)
   | val_casted_int_ptr: forall n ty attr,
       Archi.ptr64 = false -> val_casted (Vint n) (Tpointer ty attr)
-  | val_casted_ptr_int: forall b ofs si attr,
-      Archi.ptr64 = false -> val_casted (Vptr b ofs) (Tint I32 si attr)
   | val_casted_long_ptr: forall n ty attr,
       Archi.ptr64 = true -> val_casted (Vlong n) (Tpointer ty attr)
-  | val_casted_ptr_long: forall b ofs si attr,
-      Archi.ptr64 = true -> val_casted (Vptr b ofs) (Tlong si attr)
-  | val_casted_struct: forall id attr b ofs,
-      val_casted (Vptr b ofs) (Tstruct id attr)
-  | val_casted_union: forall id attr b ofs,
-      val_casted (Vptr b ofs) (Tunion id attr)
+  | val_casted_struct: forall id attr i,
+      val_casted (Vint i) (Tstruct id attr)
+  | val_casted_union: forall id attr i,
+      val_casted (Vint i) (Tunion id attr)
   | val_casted_void: forall v,
       val_casted v Tvoid.
 
@@ -1613,10 +1304,11 @@ Ltac DestructCases :=
 
 Lemma cast_val_is_casted:
   forall v ty ty' v' m, sem_cast v ty ty' m = Some v' -> val_casted v' ty'.
-Proof.
+Admitted.
+(*Proof.
   unfold sem_cast; intros.
   destruct ty, ty'; simpl in H; DestructCases; constructor; auto.
-Qed.
+Qed.*)
 
 End VAL_CASTED.
 
@@ -1636,8 +1328,6 @@ Proof.
 - auto.
 - rewrite H0; auto.
 - rewrite H0; auto.
-- rewrite H0; auto.
-- rewrite H0; auto.
 - rewrite dec_eq_true; auto.
 - rewrite dec_eq_true; auto.
 - auto. 
@@ -1654,7 +1344,8 @@ Qed.
 
 Lemma val_casted_has_type:
   forall v ty, val_casted v ty -> ty <> Tvoid -> Val.has_type v (typ_of_type ty).
-Proof.
+Admitted.
+(*Proof.
   intros. inv H; simpl typ_of_type.
 - exact I.
 - exact I.
@@ -1663,12 +1354,10 @@ Proof.
 - apply Val.Vptr_has_type.
 - red; unfold Tptr; rewrite H1; auto.
 - red; unfold Tptr; rewrite H1; auto.
-- red; unfold Tptr; rewrite H1; auto.
-- red; unfold Tptr; rewrite H1; auto.
 - apply Val.Vptr_has_type.
 - apply Val.Vptr_has_type.
 - congruence.
-Qed.
+Qed.*)
 
 (** Relation with the arithmetic conversions of ISO C99, section 6.3.1 *)
 
