cfrontend/Csyntax.v
@@ -64,7 +64,7 @@ Inductive expr : Type :=
 | Ecall (r1: expr) (rargs: exprlist) (ty: type)             (**r function call [r1(rargs)] *)
 | Ebuiltin (ef: external_function) (tyargs: typelist) (rargs: exprlist) (ty: type)
                                                                 (**r builtin function call *)
-| Eloc (b: block) (ofs: ptrofs) (pt:tag) (bf: bitfield) (ty: type)
+| Eloc (ofs: ptrofs) (pt:tag) (bf: bitfield) (ty: type)
                                       (**r memory location, result of evaluating a l-value *)
 | Eparen (r: expr) (tycast: type) (ty: type)                     (**r marked subexpression *)
 
@@ -125,7 +125,7 @@ Definition Eselection (r1 r2 r3: expr) (ty: type) :=
 
 Definition typeof (a: expr) : type :=
   match a with
-  | Eloc _ _ _ _ ty => ty
+  | Eloc _ _ _ ty => ty
   | Evar _ ty => ty
   | Ederef _ ty => ty
   | Efield _ _ ty => ty
